SIL-Parallel/Big_Step.thy
@@ -17,8 +17,8 @@ where
 Skip: "(SKIP,s) \<Down> (s, True)" |
 Abort: "(ABORT,s) \<Down> (s, False)" |
 Assign: "(x ::= a,s) \<Down> (s(x := aval a s), True)" |
-AssignND: "v \<in> S \<Longrightarrow> (x ::= ND S, s) \<Down> (s(x := aval v s), True)" |
-AssignNDEmpty: "(x ::= ND {}, s) \<Down> (s, False)" |
+AssignND: "v \<in> set S \<Longrightarrow> (x ::= ND S, s) \<Down> (s(x := aval v s), True)" |
+AssignNDEmpty: "(x ::= ND [], s) \<Down> (s, False)" |
 SeqTrue: "\<lbrakk> (c\<^sub>1,s\<^sub>1) \<Down> (s\<^sub>2,True);  (c\<^sub>2,s\<^sub>2) \<Down> sb \<rbrakk> \<Longrightarrow> (c\<^sub>1;;c\<^sub>2, s\<^sub>1) \<Down> sb" |
 SeqFalse: "\<lbrakk> (c\<^sub>1,s\<^sub>1) \<Down> (s\<^sub>2,False) \<rbrakk> \<Longrightarrow> (c\<^sub>1;;c\<^sub>2, s\<^sub>1) \<Down> (s\<^sub>2,False)" |
 IfTrue: "\<lbrakk> bval b s;  (c\<^sub>1,s) \<Down> tb \<rbrakk> \<Longrightarrow> (IF b THEN c\<^sub>1 ELSE c\<^sub>2, s) \<Down> tb" |
